exact equality with sub spec and append

VCVio/OracleComp/OracleSpec/Append.lean
@@ -38,25 +38,67 @@ This ordering is chosen to both give a generally applicable instance tree,
 and avoid an infinite typeclass search whether or not an instance exists.
 -/
 
+open OracleComp Sum
+
 namespace OracleSpec
 
-/-- `spec₁ ++ spec₂` combines the two sets of oracles disjointly using `Sum` for the indexing set.
-`Sum.inl i` is a query to oracle `i` of `spec`, and `Sum.inr i` for oracle `i` of `spec'`. -/
-@[simps] instance : Append OracleSpec where
-  append := λ spec₁ spec₂ ↦
-  { ι := spec₁.ι ⊕ spec₂.ι,
-    domain := λ i ↦ match i with
-      | Sum.inl i => spec₁.domain i
-      | Sum.inr i => spec₂.domain i,
-    range := λ i ↦ match i with
-      | Sum.inl i => spec₁.range i
-      | Sum.inr i => spec₂.range i,
-    range_inhabited' := λ i ↦ Sum.recOn i spec₁.range_inhabited spec₂.range_inhabited,
-    ι_decidableEq' := instDecidableEqSum,
-    domain_decidableEq' := λ i ↦ Sum.recOn i spec₁.domain_decidableEq spec₂.domain_decidableEq,
-    range_decidableEq' := λ i ↦ Sum.recOn i spec₁.range_decidableEq spec₂.range_decidableEq,
-    range_fintype' := λ i ↦ Sum.recOn i spec₁.range_fintype spec₂.range_fintype }
+section append
 
--- instance subSpec_append_left (spec₁ spec₂) : spec₂ ⊂ₒ (spec₁ ++ spec₂)
+/-- `spec₁ ++ spec₂` combines the two sets of oracles disjointly using `Sum` for the indexing set.
+`inl i` is a query to oracle `i` of `spec`, and `inr i` for oracle `i` of `spec'`. -/
+-- @[inline, reducible]
+def append (spec₁ spec₂ : OracleSpec) : OracleSpec where
+  ι := spec₁.ι ⊕ spec₂.ι
+  domain := λ i ↦ match i with
+    | inl i => spec₁.domain i
+    | inr i => spec₂.domain i
+  range := λ i ↦ match i with
+    | inl i => spec₁.range i
+    | inr i => spec₂.range i
+  range_inhabited' := λ i ↦ Sum.recOn i spec₁.range_inhabited spec₂.range_inhabited
+  ι_decidableEq' := Sum.instDecidableEqSum
+  domain_decidableEq' := λ i ↦ Sum.recOn i spec₁.domain_decidableEq spec₂.domain_decidableEq
+  range_decidableEq' := λ i ↦ Sum.recOn i spec₁.range_decidableEq spec₂.range_decidableEq
+  range_fintype' := λ i ↦ Sum.recOn i spec₁.range_fintype spec₂.range_fintype
+
+-- @[simp]
+instance : Append OracleSpec := ⟨OracleSpec.append⟩
+
+variable (spec₁ spec₂ : OracleSpec)
+
+end append
+
+section instances
+
+@[simps]
+instance subSpec_append_right (spec₁ spec₂ : OracleSpec) : spec₂ ⊂ₒ (spec₁ ++ spec₂) where
+  toFun := λ i t ↦ query (spec := spec₁ ++ spec₂) (inr i) t
+  evalDist_toFun' := by simp [append]; exact λ _ _ ↦ rfl
+
+@[simps]
+instance subSpec_append_left (spec₁ spec₂ : OracleSpec) : spec₁ ⊂ₒ (spec₁ ++ spec₂) where
+  toFun := λ i t ↦ query (spec := spec₁ ++ spec₂) (inl i) t
+  evalDist_toFun' := by simp [append]; exact λ _ _ ↦ rfl
+
+end instances
 
 end OracleSpec
+
+section tests
+
+variable {spec₁ spec₂ spec₃ spec₄}
+
+-- This set of examples serves as sort of a "unit test" for the coercions above
+variable (α : Type) (spec spec' spec'' spec''' : OracleSpec)
+  (coe_spec coe_spec' : OracleSpec)
+  [coe_spec ⊂ₒ coe_spec']
+
+-- coerce a single `coin_spec` and then append extra oracles
+example (oa : OracleComp coe_spec α) :
+  OracleComp (coe_spec' ++ spec' ++ spec'') α := ↑oa
+example (oa : OracleComp coe_spec α) :
+  OracleComp (spec ++ coe_spec' ++ spec') α := ↑oa
+example (oa : OracleComp coe_spec α) :
+  OracleComp (spec ++ spec' ++ coe_spec') α := ↑oa
+
+end tests
