VCVio/OracleComp/SimSemantics/Append.lean
@@ -9,7 +9,14 @@ import VCVio.OracleComp.OracleSpec.Append
 /-!
 # Append Operation for Simulation Oracles
 
-This file defines a number of basic simulation oracles, as well as operations to combine them.
+This file defines an operation `SimOracle.append` that takes two simulation oracles `so` and `so'`
+from `spec₁` and `spec₂` respectively to a shared target spec `specₜ`,
+and constructs a new simulation oracle from `spec₁ ++ spec₂` to `specₜ`.
+
+This operation is also compatible with the `SubSpec` instances involving `OracleSpec.append`.
+For example if `oa : OracleComp spec₁ α` is coerced to `↑oa : OracleComp (spec₁ ++ spec₂) α`,
+then we have `simulate' (so ++ₛₒ so') ↑oa s = simulate' so oa s.1`, as the additional
+oracles from the coercion will never actually be called.
 -/
 
 open OracleSpec OracleComp Prod Sum
@@ -42,5 +49,26 @@ lemma append_apply_inl (so : spec₁ →[σ]ₛₒ specₜ) (so' : spec₂ →[�
 lemma append_apply_inr (so : spec₁ →[σ]ₛₒ specₜ) (so' : spec₂ →[τ]ₛₒ specₜ)
     (i : spec₂.ι) : (so ++ₛₒ so') (inr i) = λ ⟨t, s₁, s₂⟩ ↦ do
       let ⟨u, s₂'⟩ ← so' i (t, s₂) return (u, s₁, s₂') := rfl
+
+section subSpec
+
+@[simp]
+lemma simulate_coe_append_left (so : spec₁ →[σ]ₛₒ specₜ) (so' : spec₂ →[τ]ₛₒ specₜ)
+    (oa : OracleComp spec₁ α) (s : σ × τ) :
+    simulate (so ++ₛₒ so') ↑oa s = (λ ⟨x, s'⟩ ↦ (x, (s', s.2))) <$> simulate so oa s.1 := by
+  revert s
+  induction oa using OracleComp.inductionOn with
+  | h_pure x => simp
+  | h_query_bind i t oa hoa => simp [hoa, map_bind]
+
+@[simp]
+lemma simulate'_coe_append_left (so : spec₁ →[σ]ₛₒ specₜ) (so' : spec₂ →[τ]ₛₒ specₜ)
+    (oa : OracleComp spec₁ α) (s : σ × τ) :
+    simulate' (so ++ₛₒ so') ↑oa s = simulate' so oa s.1 := by
+  rw [simulate'_def (so ++ₛₒ so'), simulate_coe_append_left, Functor.map_map,
+    Function.comp, simulate'_def]
+
+
+end subSpec
 
 end append
